Work on writing Fourier-Motzkin projection

CodeGen.v
@@ -1,5 +1,6 @@
 Require Import String.
 
+Require Import QArith.
 Require Import ZArith.
 Require Import List.
 Require Import Bool.
@@ -268,14 +269,21 @@ Proof.
   - intros H; split; intros c Hin Hcmp; apply H; auto; lia.
 Qed.
 
+(*
+Require Import Vpl.DomainInterfaces.
+Require Import Vpl.ConsSet.
+Require Import Vpl.PedraQ.
+Require Import VplInterface.
+ *)
+Require Import Vpl.Impure.
 
 (** * Polyhedral projection, using an untrusted oracle and a certificate *)
 
-Module Type PolyProject.
-  Parameter project : nat -> polyhedron -> result polyhedron.
+Module Type PolyProject (Import Imp: FullImpureMonad).
+  Parameter project : nat * polyhedron -> imp polyhedron.
 
   Parameter project_inclusion :
-    forall n p pol proj, project n pol = Ok proj -> in_poly p pol = true -> in_poly (resize n p) proj = true.
+    forall n p pol, in_poly p pol = true -> WHEN proj <- project (n, pol) THEN in_poly (resize n p) proj = true.
 
   Parameter project_invariant : nat -> polyhedron -> list Z -> Prop.
 
@@ -286,19 +294,21 @@ Module Type PolyProject.
     forall n pol p, (forall c, In c pol -> fst c =v= resize n (fst c)) -> project_invariant n pol p -> in_poly p pol = true.
 
   Parameter project_next_r_inclusion :
-    forall n pol proj p, project (S n) pol = Ok proj -> project_invariant n pol p ->
-                    (forall c, In c proj -> nth n (fst c) 0 <> 0 -> satisfies_constraint p c = true) -> project_invariant (S n) pol p.
+    forall n pol p, project_invariant n pol p ->
+               WHEN proj <- project (S n, pol) THEN
+               (forall c, In c proj -> nth n (fst c) 0 <> 0 -> satisfies_constraint p c = true) ->
+                 project_invariant (S n) pol p.
 
   Parameter project_invariant_resize :
     forall n pol p, project_invariant n pol p <-> project_invariant n pol (resize n p).
 
-  Parameter project_invariant_export : nat -> polyhedron -> result polyhedron.
+  Parameter project_invariant_export : nat * polyhedron -> imp polyhedron.
 
   Parameter project_invariant_export_correct :
-    forall n p pol res, project_invariant_export n pol = Ok res -> in_poly p res = true <-> project_invariant n pol p.
+    forall n p pol, WHEN res <- project_invariant_export (n, pol) THEN in_poly p res = true <-> project_invariant n pol p.
 
   Parameter project_constraint_size :
-    forall n pol proj c, project n pol = Ok proj -> In c proj -> fst c =v= resize n (fst c).
+    forall n pol c, WHEN proj <- project (n, pol) THEN In c proj -> fst c =v= resize n (fst c).
 
 End PolyProject.
 
@@ -307,35 +317,45 @@ Ltac destruct_if H Heq :=
     | [ H : context[if ?X then _ else _] |- _ ] => destruct X eqn:Heq
   end.
 
-Module PolyProjectSimple <: PolyProject.
+Ltac destruct_if_g Heq :=
+  lazymatch goal with
+    | [ |- context[if ?X then _ else _] ] => destruct X eqn:Heq
+  end.
+
+Require Vpl.ImpureConfig.
+
+Module CoreAlarmed := AlarmImpureMonad Vpl.ImpureConfig.Core.
+
+Module PolyProjectSimple (Import Imp: FullAlarmedMonad) <: PolyProject Imp.
 
   Parameter untrusted_project : nat -> polyhedron -> (polyhedron * list witness)%type.
 
-  Definition project n p :=
+  Definition project (np : nat * polyhedron) : imp polyhedron :=
+    let (n, p) := np in
     let (res, wits) := untrusted_project n p in
     if negb (length res =? length wits)%nat then
-      Err "Incorrect number of witnesses"
+      alarm "Incorrect number of witnesses" p
     else if negb (forallb (fun c => is_eq (fst c) (resize n (fst c))) res) then
-      Err "Constraint too long"
+      alarm "Constraint too long" p
     else if negb (forallb (fun z => is_redundant (snd z) p (fst z)) (combine res wits)) then
-      Err "Witness checking failed"
+      alarm "Witness checking failed" p
     else if negb (forallb (fun c => negb (is_eq (fst c) (resize n (fst c))) || existsb (fun c' => is_eq (fst c) (fst c') && (snd c =? snd c')) res) p) then
-      Err "Constraint removed in projection"
+      alarm "Constraint removed in projection" p
     else
-      Ok res.
+      pure res.
 
   Theorem project_inclusion :
-    forall n p pol proj, project n pol = Ok proj -> in_poly p pol = true -> in_poly (resize n p) proj = true.
+    forall n p pol, in_poly p pol = true -> WHEN proj <- project (n, pol) THEN in_poly (resize n p) proj = true.
   Proof.
-    intros n p pol proj Hok Hin.
-    unfold project in Hok.
+    intros n p pol Hin.
+    unfold project.
     destruct (untrusted_project n pol) as [res wits].
-    destruct_if Hok Hlen; reflect; [congruence|].
-    destruct_if Hok Hresize; reflect; [congruence|].
-    destruct_if Hok Hwits; reflect; [congruence|].
-    destruct_if Hok Hpreserve; reflect; [congruence|].
-    injection Hok as Hok; rewrite Hok in *.
-    assert (Hinproj : in_poly p proj = true).
+    destruct_if_g Hlen; reflect; [xasimplify ltac:(eauto using mayReturn_alarm)|].
+    destruct_if_g Hresize; reflect; [xasimplify ltac:(eauto using mayReturn_alarm)|].
+    destruct_if_g Hwits; reflect; [xasimplify ltac:(eauto using mayReturn_alarm)|].
+    destruct_if_g Hpreserve; reflect; [xasimplify ltac:(eauto using mayReturn_alarm)|].
+    xasimplify eauto.
+    assert (Hinres : in_poly p res = true).
     - unfold in_poly. rewrite forallb_forall. intros c Hc.
       apply in_l_combine with (l' := wits) in Hc; [|auto].
       destruct Hc as [wit Hwit].
@@ -343,7 +363,7 @@ Module PolyProjectSimple <: PolyProject.
       rewrite forallb_forall in Hwits.
       apply (Hwits (c, wit)); auto.
     - unfold in_poly in *. rewrite forallb_forall in *. intros c Hc.
-      rewrite <- (Hinproj c) by auto.
+      rewrite <- (Hinres c) by auto.
       unfold satisfies_constraint. f_equal. specialize (Hresize c Hc). reflect.
       rewrite Hresize.
       rewrite <- dot_product_resize_left with (t1 := p). rewrite resize_length. reflexivity.
@@ -353,16 +373,16 @@ Module PolyProjectSimple <: PolyProject.
     forall c, In c pol -> fst c =v= resize n (fst c) -> satisfies_constraint p c = true.
 
   Theorem project_reverse_inclusion :
-    forall n pol proj c, project n pol = Ok proj -> In c pol -> fst c =v= resize n (fst c) -> (exists c', c =c= c' /\ In c' proj).
+    forall n pol c, In c pol -> fst c =v= resize n (fst c) -> WHEN proj <- project (n, pol) THEN (exists c', c =c= c' /\ In c' proj).
   Proof.
-    intros n pol proj c Hok Hin Heq.
-    unfold project in Hok.
+    intros n pol c Hin Heq.
+    unfold project.
     destruct (untrusted_project n pol) as [res wits].
-    destruct_if Hok Hlen; reflect; [congruence|].
-    destruct_if Hok Hresize; reflect; [congruence|].
-    destruct_if Hok Hwits; reflect; [congruence|].
-    destruct_if Hok Hpreserve; reflect; [congruence|].
-    injection Hok as Hok; rewrite Hok in *.
+    destruct_if_g Hlen; reflect; [xasimplify ltac:(exfalso; eauto using mayReturn_alarm)|].
+    destruct_if_g Hresize; reflect; [xasimplify ltac:(exfalso; eauto using mayReturn_alarm)|].
+    destruct_if_g Hwits; reflect; [xasimplify ltac:(exfalso; eauto using mayReturn_alarm)|].
+    destruct_if_g Hpreserve; reflect; [xasimplify ltac:(exfalso; eauto using mayReturn_alarm)|].
+    xasimplify eauto.
     reflect_binders.
     specialize (Hpreserve c Hin).
     rewrite <- is_eq_veq in Heq; rewrite Heq in Hpreserve.
@@ -389,16 +409,18 @@ Module PolyProjectSimple <: PolyProject.
   Qed.
 
   Theorem project_next_r_inclusion :
-    forall n pol proj p, project (S n) pol = Ok proj -> project_invariant n pol p ->
-                    (forall c, In c proj -> nth n (fst c) 0 <> 0 -> satisfies_constraint p c = true) -> project_invariant (S n) pol p.
+    forall n pol p, project_invariant n pol p ->
+               WHEN proj <- project (S n, pol) THEN
+                 (forall c, In c proj -> nth n (fst c) 0 <> 0 -> satisfies_constraint p c = true) ->
+                 project_invariant (S n) pol p.
   Proof.
-    intros n pol proj p Hproj Hinv Hsat c Hcin Hclen.
+    intros n pol p Hinv proj Hproj Hsat c Hcin Hclen.
     destruct (nth n (fst c) 0 =? 0) eqn:Hzero; reflect.
     - rewrite resize_succ in Hclen. rewrite Hzero in Hclen.
-      setoid_replace (0 :: nil) with (@nil Z) in Hclen by (rewrite <- is_eq_veq; auto).
+      setoid_replace (0 :: nil) with (@nil Z) using relation veq in Hclen by (rewrite <- is_eq_veq; auto).
       rewrite app_nil_r in Hclen.
       apply Hinv; auto.
-    - destruct (project_reverse_inclusion (S n) pol proj c Hproj Hcin Hclen) as [c' [Heqc' Hc'in]].
+    - destruct (project_reverse_inclusion (S n) pol c Hcin Hclen proj Hproj) as [c' [Heqc' Hc'in]].
       rewrite Heqc'. apply Hsat; auto. erewrite nth_eq; eauto. rewrite Heqc'; reflexivity.
   Qed.
 
@@ -412,39 +434,711 @@ Module PolyProjectSimple <: PolyProject.
     rewrite Hclen. rewrite <- dot_product_resize_left. rewrite resize_length; auto.
   Qed.
 
-  Definition project_invariant_export n (pol : polyhedron) :=
-    Ok (filter (fun c => is_eq (fst c) (resize n (fst c))) pol).
+  Definition project_invariant_export (np : nat * polyhedron) : imp polyhedron :=
+    pure (filter (fun c => is_eq (fst c) (resize (fst np) (fst c))) (snd np)).
 
   Theorem project_invariant_export_correct :
-    forall n p pol res, project_invariant_export n pol = Ok res -> in_poly p res = true <-> project_invariant n pol p.
+    forall n p pol, WHEN res <- project_invariant_export (n, pol) THEN in_poly p res = true <-> project_invariant n pol p.
   Proof.
-    intros n p pol res Heq. unfold project_invariant_export in Heq; injection Heq as Heq.
-    rewrite <- Heq in *. unfold project_invariant. unfold in_poly.
+    intros n p pol. xasimplify eauto.
+    unfold project_invariant. unfold in_poly.
     rewrite forallb_forall. under_forall ((list Z * Z)%type) ltac:(fun x => rewrite filter_In; reflect).
     firstorder.
   Qed.
 
   Theorem project_constraint_size :
-    forall n pol proj c, project n pol = Ok proj -> In c proj -> fst c =v= resize n (fst c).
+    forall n pol c, WHEN proj <- project (n, pol) THEN In c proj -> fst c =v= resize n (fst c).
   Proof.
-    intros n pol proj c Hproj Hin.
-    unfold project in Hproj.
+    intros n pol c. unfold project.
     destruct (untrusted_project n pol) as [res wits].
-    destruct_if Hproj Hlen; [congruence|].
-    destruct_if Hproj Hresize; [congruence|].
-    destruct_if Hproj Hwits; [congruence|].
-    destruct_if Hproj Hpreserve; [congruence|].
-    injection Hproj as Hproj; rewrite Hproj in *.
-    reflect. rewrite forallb_forall in Hresize. specialize (Hresize c); reflect; eauto.
+    destruct_if_g Hlen; reflect; [xasimplify ltac:(exfalso; eauto using mayReturn_alarm)|].
+    destruct_if_g Hresize; reflect; [xasimplify ltac:(exfalso; eauto using mayReturn_alarm)|].
+    destruct_if_g Hwits; reflect; [xasimplify ltac:(exfalso; eauto using mayReturn_alarm)|].
+    destruct_if_g Hpreserve; reflect; [xasimplify ltac:(exfalso; eauto using mayReturn_alarm)|].
+    xasimplify eauto.
+    reflect. intros Hin.
+    rewrite forallb_forall in Hresize. specialize (Hresize c); reflect; eauto.
   Qed.
 
 End PolyProjectSimple.
 
-Require Import Vpl.DomainInterfaces.
-Require Import Vpl.ConsSet.
-Require Import Vpl.PedraQ.
 Require Import VplInterface.
 
+
+Definition assign n x v :=
+  resize n v ++ (x :: (skipn (S n) v)).
+
+Definition mult_constraint_cst k (c : (list Z * Z)) := (fst c, k * snd c).
+
+Definition expand_poly k pol := map (mult_constraint_cst k) pol.
+
+Module Type PolyCanonizer (Import Imp: FullImpureMonad).
+
+  Parameter canonize : polyhedron -> imp polyhedron.
+
+  Parameter canonize_correct :
+    forall p, WHEN r <- canonize p THEN (forall k v, 0 < k -> in_poly v (expand_poly k r) = in_poly v (expand_poly k p)).
+
+  Parameter canonize_no_new_var :
+    forall k p, (forall c, In c p -> nth k (fst c) 0 = 0) -> WHEN r <- canonize p THEN (forall c, In c r -> nth k (fst c) 0 = 0).
+
+End PolyCanonizer.
+
+Module NaiveCanonizer(Import Imp: FullImpureMonad) <: PolyCanonizer Imp.
+
+  Definition canonize (p : polyhedron) := pure p.
+
+  Theorem canonize_correct :
+    forall p, WHEN r <- canonize p THEN (forall k v, 0 < k -> in_poly v (expand_poly k r) = in_poly v (expand_poly k p)).
+  Proof.
+    intros p r Hcanon k v Hk. unfold canonize in Hcanon.
+    apply mayReturn_pure in Hcanon. rewrite Hcanon. reflexivity.
+  Qed.
+
+  Theorem canonize_no_new_var :
+    forall k p, (forall c, In c p -> nth k (fst c) 0 = 0) -> WHEN r <- canonize p THEN (forall c, In c r -> nth k (fst c) 0 = 0).
+  Proof.
+    intros k p H r Hcanon. unfold canonize in Hcanon.
+    apply mayReturn_pure in Hcanon. rewrite Hcanon in H. exact H.
+  Qed.
+
+End NaiveCanonizer.
+
+Module Type ProjectOperator (Import Imp: FullImpureMonad).
+
+  Parameter project : (nat * polyhedron) -> imp polyhedron.
+
+  Parameter project_projected :
+    forall n pol, WHEN proj <- project (n, pol) THEN forall c, In c proj -> nth n (fst c) 0 = 0.
+
+  Parameter project_no_new_var :
+    forall n k pol, (forall c, In c pol -> nth k (fst c) 0 = 0) -> WHEN proj <- project (n, pol) THEN (forall c, In c proj -> nth k (fst c) 0 = 0).
+
+  Parameter project_in_iff :
+    forall n p pol s, 0 < s ->
+                 WHEN proj <- project (n, pol) THEN
+                      in_poly p (expand_poly s proj) = true <->
+                 exists t k, 0 < t /\ in_poly (assign n k (mult_vector t p)) (expand_poly (s * t) pol) = true.
+
+End ProjectOperator.
+
+Require Import QOrderedType.
+
+Module FourierMotzkinProject (Import Imp: FullImpureMonad) <: ProjectOperator Imp.
+
+  Definition merge_constraints n c1 c2 :=
+    let '(g, (aa, bb)) := Z.ggcd (nth n (fst c1) 0) (nth n (fst c2) 0) in
+    add_constraint (mult_constraint bb c1) (mult_constraint_cst (-aa) c2).
+
+  Lemma Q_exists_rec :
+    forall (l1 l2 : list Q) (y1 : Q), ((exists x : Q, (forall y : Q, In y l1 -> (y <= x)%Q) /\ (forall z : Q, In z l2 -> (x <= z)%Q)) <->
+                                  (forall y z : Q, In y l1 -> In z l2 -> (y <= z)%Q)) ->
+                                 ((exists x : Q, (forall y : Q, In y (y1 :: l1) -> (y <= x)%Q) /\ (forall z : Q, In z l2 -> (x <= z)%Q)) <->
+                                  (forall y z : Q, In y (y1 :: l1) -> In z l2 -> (y <= z)%Q)).
+  Proof.
+    intros l1 l2 y1 [Himp1 Himp2].
+    split.
+    - intros [x [Hxy Hxz]] y z Hiny Hinz.
+      specialize (Hxy y Hiny). specialize (Hxz z Hinz). q_order.
+    - intros H. destruct Himp2 as [x [Hxy Hxz]].
+      + intros y z Hiny Hinz. apply H; simpl; auto.
+      + destruct (Qlt_le_dec x y1).
+        * exists y1. split.
+          -- intros y [Hy1| Hiny]; [rewrite Hy1 | specialize (Hxy y Hiny)]; q_order.
+          -- intros z Hinz. apply H; simpl; auto.
+        * exists x. split.
+          -- intros y [Hy1 | Hiny]; [rewrite Hy1 in *; q_order | apply Hxy; auto].
+          -- auto.
+  Qed.
+
+  Lemma Q_exists_min :
+    forall (l : list Q), exists x : Q, forall y : Q, In y l -> (x <= y)%Q.
+  Proof.
+    induction l as [|y1 l IH].
+    - exists 0%Q; intros; simpl in *; tauto.
+    - destruct IH as [x IH].
+      destruct (Qlt_le_dec x y1).
+      + exists x. intros y [Hy1 | Hiny]; [rewrite Hy1 in *; q_order | apply (IH y Hiny)].
+      + exists y1. intros y [Hy1 | Hiny]; [rewrite Hy1 | specialize (IH y Hiny)]; q_order.
+  Qed.
+
+
+  Lemma Q_exists_between :
+    forall (l1 l2 : list Q), (exists x : Q, (forall y : Q, In y l1 -> (y <= x)%Q) /\ (forall z : Q, In z l2 -> (x <= z)%Q)) <->
+                        (forall y z : Q, In y l1 -> In z l2 -> (y <= z)%Q).
+  Proof.
+    induction l1 as [|y1 l1 IH1].
+    - intros l2. split.
+      + intros; simpl in *; tauto.
+      + intros H; destruct (Q_exists_min l2) as [x Hx]; exists x.
+        split; [intros; simpl in *; tauto | apply Hx].
+    - intros l2; apply Q_exists_rec. apply IH1.
+  Qed.
+  
+
+End FourierMotzkinProject.
+
+
+Fixpoint list_max l :=
+  match l with
+  | nil => 0%nat
+  | x :: l => Nat.max x (list_max l)
+  end.
+
+Theorem list_max_le :
+  forall l n, (list_max l <= n -> (forall x, In x l -> x <= n))%nat.
+Proof.
+  induction l; simpl in *.
+  - intros; exfalso; auto.
+  - intros n H x [Ha | Hl].
+    + lia.
+    + apply IHl; auto; lia.
+Qed.
+
+Theorem list_le_max :
+  forall l n, (forall x, In x l -> x <= n)%nat -> (list_max l <= n)%nat.
+Proof.
+  induction l; simpl in *.
+  - intros; lia.
+  - intros n H. apply Nat.max_lub.
+    + apply H; auto.
+    + apply IHl; intros; apply H; auto.
+Qed.
+
+Theorem list_max_def :
+  forall l n, (list_max l <= n <-> (forall x, In x l -> x <= n))%nat.
+Proof.
+  intros l n; split; [apply list_max_le | apply list_le_max].
+Qed.
+
+Lemma mult_vector_1 :
+  forall v, mult_vector 1 v = v.
+Proof.
+  induction v; simpl; auto; destruct a; auto.
+Qed.
+
+Lemma mult_constraint_1 :
+  forall c, mult_constraint 1 c = c.
+Proof.
+  intros c; destruct c as [v x]; unfold mult_constraint.
+  simpl in *; rewrite mult_vector_1.
+  f_equal; destruct x; auto.
+Qed.
+
+Lemma mult_constraint_cst_1 :
+  forall c, mult_constraint_cst 1 c = c.
+Proof.
+  intros c; destruct c as [v x]; destruct x; auto.
+Qed.
+
+Lemma expand_poly_1 :
+  forall p, expand_poly 1 p = p.
+Proof.
+  intros p.
+  unfold expand_poly. erewrite map_ext; [apply map_id|].
+  apply mult_constraint_cst_1.
+Qed.
+
+Lemma mult_vector_resize :
+  forall n k v, resize n (mult_vector k v) = mult_vector k (resize n v).
+Proof.
+  induction n.
+  - intros; simpl in *; auto.
+  - intros; simpl in *.
+    destruct v; simpl in *; rewrite <- IHn; f_equal.
+    lia.
+Qed.
+
+Lemma mult_vector_skipn :
+  forall n k v, skipn n (mult_vector k v) = mult_vector k (skipn n v).
+Proof.
+  induction n.
+  - intros; simpl in *; auto.
+  - intros; destruct v; simpl in *; auto.
+Qed.
+
+Lemma mult_constraint_cst_eq :
+  forall c k p, 0 < k -> satisfies_constraint (mult_vector k p) (mult_constraint_cst k c) = satisfies_constraint p c.
+Proof.
+  intros c k p Hk.
+  unfold satisfies_constraint, mult_constraint_cst.
+  rewrite dot_product_mult_left. simpl.
+  apply eq_iff_eq_true. reflect.
+  nia.
+Qed.
+
+Lemma expand_poly_eq :
+  forall p k v, 0 < k -> in_poly (mult_vector k v) (expand_poly k p) = in_poly v p.
+Proof.
+  intros p k v Hk.
+  unfold in_poly, expand_poly. rewrite forallb_map. apply forallb_ext.
+  intros; apply mult_constraint_cst_eq; auto.
+Qed.
+
+Lemma mult_constraint_cst_comp :
+  forall s t c, mult_constraint_cst s (mult_constraint_cst t c) = mult_constraint_cst (s * t) c.
+Proof.
+  intros. unfold mult_constraint_cst. simpl. f_equal.
+  nia.
+Qed.
+
+Lemma expand_poly_comp :
+  forall s t p, expand_poly s (expand_poly t p) = expand_poly (s * t) p.
+Proof.
+  intros. unfold expand_poly.
+  rewrite map_map. apply map_ext.
+  apply mult_constraint_cst_comp.
+Qed.
+
+Lemma mult_vector_comp :
+  forall s t v, mult_vector s (mult_vector t v) = mult_vector (s * t) v.
+Proof.
+  intros s t v. unfold mult_vector. rewrite map_map; apply map_ext.
+  intros; nia.
+Qed.
+
+Lemma mult_vector_app :
+  forall s v1 v2, mult_vector s (v1 ++ v2) = mult_vector s v1 ++ mult_vector s v2.
+Proof.
+  intros s v1 v2. unfold mult_vector. apply map_app.
+Qed.
+
+Lemma resize_app_ge :
+  forall n v1 v2, (n <= length v1)%nat -> resize n (v1 ++ v2) = resize n v1.
+Proof.
+  induction n.
+  - intros; simpl in *; auto.
+  - intros; destruct v1; simpl in *; [|rewrite IHn]; auto; lia.
+Qed.
+
+Lemma skipn_app_le :
+  forall (A : Type) n (v1 v2 : list A), (length v1 <= n)%nat -> skipn n (v1 ++ v2) = skipn (n - length v1) v2.
+Proof.
+  intros A n; induction n.
+  - intros; simpl in *.
+    destruct v1; simpl in *; auto; lia.
+  - intros v1 v2 H; destruct v1.
+    + reflexivity.
+    + simpl in *; apply IHn; lia.
+Qed.
+
+Lemma skipn_app_ge :
+  forall (A : Type) n (v1 v2 : list A), (n <= length v1)%nat -> skipn n (v1 ++ v2) = skipn n v1 ++ v2.
+Proof.
+  intros A n; induction n.
+  - intros; simpl; auto.
+  - intros; destruct v1; simpl in *; [|apply IHn]; lia.
+Qed.
+
+Lemma assign_app_lt :
+  forall n k v1 v2, (n < length v1)%nat -> assign n k (v1 ++ v2) = assign n k v1 ++ v2.
+Proof.
+  intros n k v1 v2 H. unfold assign.
+  rewrite <- app_assoc. rewrite skipn_app_ge by lia. rewrite resize_app_ge by lia.
+  reflexivity.
+Qed.
+
+Lemma assign_app_ge :
+  forall n k v1 v2, (length v1 <= n)%nat -> assign n k (v1 ++ v2) = v1 ++ assign (n - length v1) k v2.
+Proof.
+  intros n k v1 v2 H. unfold assign.
+  rewrite resize_app_le by lia. rewrite skipn_app_le by lia. rewrite <- app_assoc.
+  f_equal. f_equal. f_equal. f_equal. lia.
+Qed.
+
+Lemma resize_length_eq :
+  forall n l, length l = n -> resize n l = l.
+Proof.
+  induction n; intros; destruct l; simpl in *; auto; lia.
+Qed.
+
+Fixpoint nrlength l :=
+  match l with
+  | nil => 0%nat
+  | x :: l => let n := nrlength l in if (x =? 0) && (n =? 0)%nat then 0%nat else S n
+  end.
+
+Lemma nrlength_zero_null :
+  forall l, nrlength l = 0%nat -> is_null l = true.
+Proof.
+  induction l.
+  - simpl in *; auto.
+  - intros H; simpl in *.
+    destruct (a =? 0); simpl in *; [|congruence].
+    destruct (nrlength l); simpl in *; [auto|congruence].
+Qed.
+
+Lemma nrlength_null_zero :
+  forall l, is_null l = true -> nrlength l = 0%nat.
+Proof.
+  induction l.
+  - simpl; auto.
+  - intros H; simpl in *; reflect; destruct H as [H1 H2]; rewrite IHl by auto; rewrite H1; reflexivity.
+Qed.
+
+Lemma nrlength_zero_null_iff :
+  forall l, nrlength l = 0%nat <-> is_null l = true.
+Proof.
+  intros l; split; [apply nrlength_zero_null | apply nrlength_null_zero].
+Qed.
+
+Lemma nrlength_def :
+  forall l n, resize n l =v= l <-> (nrlength l <= n)%nat.
+Proof.
+  induction l.
+  - intros n; simpl in *. split; intros; [lia|].
+    rewrite <- is_eq_veq. rewrite is_eq_nil_right. apply resize_nil_null.
+  - intros n. rewrite <- is_eq_veq. destruct n.
+    + simpl in *. destruct (a =? 0); simpl; [|split; intros; [congruence|lia]].
+      rewrite <- nrlength_zero_null_iff.
+      destruct (nrlength l); simpl in *; split; intros; lia.
+    + simpl. rewrite Z.eqb_refl. simpl. rewrite is_eq_veq. rewrite IHl.
+      destruct_if_g H; reflect; lia.
+Qed.
+
+Lemma nrlength_eq :
+  forall l, resize (nrlength l) l =v= l.
+Proof.
+  intros; rewrite nrlength_def; lia.
+Qed.
+
+Lemma nrlength_def_impl :
+  forall l n, (nrlength l <= n)%nat -> resize n l =v= l.
+Proof.
+  intros; rewrite nrlength_def; auto.
+Qed.
+
+Lemma dot_product_nrlength_right :
+  forall v1 v2 n, (nrlength v1 <= n)%nat -> dot_product v1 (resize n v2) = dot_product v1 v2.
+Proof.
+  intros v1 v2 n H. rewrite <- (nrlength_def_impl v1 n) by auto.
+  rewrite <- dot_product_resize_right with (t2 := v2). rewrite resize_length. reflexivity.
+Qed.
+
+Lemma dot_product_nrlength_left :
+  forall v1 v2 n, (nrlength v2 <= n)%nat -> dot_product (resize n v1) v2 = dot_product v1 v2.
+Proof.
+  intros v1 v2 n H. rewrite dot_product_commutative. rewrite dot_product_nrlength_right by auto.
+  apply dot_product_commutative.
+Qed.
+
+Lemma satisfies_constraint_nrlength :
+  forall p c n, (nrlength (fst c) <= n)%nat -> satisfies_constraint (resize n p) c = satisfies_constraint p c.
+Proof.
+  intros p c n H. unfold satisfies_constraint.
+  rewrite dot_product_nrlength_left; auto.
+Qed.
+
+Definition poly_nrl (pol : polyhedron) := list_max (map (fun c => nrlength (fst c)) pol).
+
+Lemma in_poly_nrlength :
+  forall p pol n, (poly_nrl pol <= n)%nat -> in_poly (resize n p) pol = in_poly p pol.
+Proof.
+  intros p pol n H.
+  unfold in_poly. rewrite eq_iff_eq_true, !forallb_forall. apply forall_ext.
+  intros c.
+  enough (In c pol -> satisfies_constraint (resize n p) c = satisfies_constraint p c) by (intuition congruence).
+  intros Hin. apply satisfies_constraint_nrlength.
+  eapply list_max_le; [exact H|]. rewrite in_map_iff. exists c. auto.
+Qed.
+
+Lemma nrlength_mult :
+  forall k v, k <> 0 -> nrlength (mult_vector k v) = nrlength v.
+Proof.
+  intros k. induction v.
+  - simpl; auto.
+  - intros; simpl. rewrite IHv by auto.
+    replace (k * a =? 0) with (a =? 0); [reflexivity|].
+    rewrite eq_iff_eq_true; reflect; nia.
+Qed.
+
+Lemma expand_poly_nrl :
+  forall k p, k <> 0 -> poly_nrl (expand_poly k p) = poly_nrl p.
+Proof.
+  intros k p H. unfold poly_nrl, expand_poly.
+  rewrite map_map. f_equal.
+Qed.
+
+Lemma poly_nrl_def :
+  forall n pol, (forall c, In c pol -> fst c =v= resize n (fst c)) <-> (poly_nrl pol <= n)%nat.
+Proof.
+  intros n pol. unfold poly_nrl. rewrite list_max_def. split.
+  - intros H x Hin. rewrite in_map_iff in Hin. destruct Hin as [c [Hlen Hin]].
+    rewrite <- Hlen, <- nrlength_def. symmetry; auto.
+  - intros H c Hin. symmetry; rewrite nrlength_def. apply H.
+    rewrite in_map_iff; exists c; auto.
+Qed.
+
+Lemma nth_resize :
+  forall n k v, nth k (resize n v) 0 = if (k <? n)%nat then nth k v 0 else 0.
+Proof.
+  induction n.
+  - intros k v; destruct k; auto.
+  - intros k v; destruct k; destruct v; simpl; auto;
+      replace (S k <? S n)%nat with (k <? n)%nat by (rewrite eq_iff_eq_true; reflect; lia); rewrite IHn; destruct k; reflexivity.
+Qed.
+
+Module PolyProjectImpl (Import Imp: FullImpureMonad) (Canon : PolyCanonizer Imp) (Proj : ProjectOperator Imp) <: PolyProject Imp.
+
+  Ltac bind_imp_destruct H id1 id2 :=
+  apply mayReturn_bind in H; destruct H as [id1 [id2 H]].
+
+  Fixpoint do_project d k pol :=
+    match k with
+    | O => pure pol
+    | S k1 =>
+      BIND proj <- Proj.project ((d + k1)%nat, pol) -;
+      BIND canon <- Canon.canonize proj -;
+      do_project d k1 canon
+    end.
+
+  Lemma do_project_succ :
+    forall k d pol, impeq (do_project d (S k) pol)
+                     (BIND proj1 <- do_project (S d) k pol -; BIND proj <- Proj.project (d, proj1) -; Canon.canonize proj).
+  Proof.
+    induction k.
+    - intros; simpl in *. rewrite Nat.add_0_r.
+      rewrite impeq_bind_pure_l. f_equiv; intro proj1. rewrite impeq_bind_pure_r. reflexivity.
+    - intros d pol; simpl in *.
+      rewrite impeq_bind_assoc. rewrite Nat.add_succ_r. f_equiv; intro proj.
+      rewrite impeq_bind_assoc. f_equiv; intro canon.
+      rewrite IHk. reflexivity.
+  Qed.
+
+  Lemma do_project_in_iff :
+    forall k s d p pol, 0 < s ->
+                   WHEN proj <- do_project d k pol THEN
+                        in_poly p (expand_poly s proj) = true <->
+                   exists t m, length m = k /\ 0 < t /\
+                          in_poly (resize d (mult_vector t p) ++ m ++ skipn (d + k)%nat (mult_vector t p))
+                                  (expand_poly (s * t) pol) = true.
+  Proof.
+    induction k.
+    - intros s d p pol Hs proj Hproj; simpl in *.
+      apply mayReturn_pure in Hproj; rewrite Hproj.
+      split.
+      + intros Hin. exists 1. exists nil. simpl.
+        split; [auto|split;[lia|]].
+        rewrite !mult_vector_1, Nat.add_0_r, resize_skipn_eq, Z.mul_1_r.
+        exact Hin.
+      + intros [t [m [Hm [Ht Hin]]]].
+        destruct m; simpl in *; [|congruence].
+        rewrite Nat.add_0_r, resize_skipn_eq, Z.mul_comm, <- expand_poly_comp, expand_poly_eq in Hin by auto.
+        exact Hin.
+    - intros s d p pol Hs proj Hproj; simpl in *.
+      bind_imp_destruct Hproj proja Hproja.
+      bind_imp_destruct Hproj canon Hcanon.
+      rewrite (IHk s d p canon Hs proj Hproj).
+      split; intros [t [m [Hmlen [Ht Hin]]]]; assert (Hst : 0 < s * t) by nia.
+      + rewrite (Canon.canonize_correct proja) in Hin by auto.
+        rewrite (Proj.project_in_iff _ _ _ _ Hst _ Hproja) in Hin.
+        destruct Hin as [r [u [Hr Hin]]].
+        exists (t * r). exists (mult_vector r m ++ (u :: nil)).
+        split; [rewrite app_length, mult_vector_length, Nat.add_1_r; auto|].
+        split; [nia|].
+        rewrite <- Hin, Z.mul_assoc. f_equiv.
+        rewrite !mult_vector_app, <- !mult_vector_resize, <- !mult_vector_skipn, !mult_vector_comp.
+        rewrite assign_app_ge; rewrite resize_length; [|lia].
+        rewrite assign_app_ge; rewrite mult_vector_length, Hmlen; [|lia].
+        replace (d + k - d - k)%nat with 0%nat by lia.
+        rewrite <- app_assoc.
+        f_equiv; [f_equal; f_equal; nia|].
+        f_equiv. unfold assign. rewrite skipn_skipn. replace (1 + (d + k))%nat with (d + S k)%nat by lia.
+        simpl. f_equiv. f_equiv. f_equal. nia.
+      + exists t. exists (resize k m). split; [apply resize_length|].
+        split; [auto|].
+        rewrite (Canon.canonize_correct proja) by auto.
+        rewrite (Proj.project_in_iff _ _ _ _ Hst _ Hproja).
+        exists 1. exists (nth k m 0).
+        split; [lia|].
+        rewrite mult_vector_1. rewrite <- Hin.
+        f_equiv; [|f_equal; lia].
+        rewrite assign_app_ge; rewrite resize_length; [|lia].
+        rewrite assign_app_ge; rewrite resize_length; [|lia].
+        replace (d + k - d - k)%nat with 0%nat by lia.
+        unfold assign.
+        rewrite skipn_skipn. replace (1 + (d + k))%nat with (d + S k)%nat by lia.
+        replace m with (resize k m ++ (nth k m 0 :: nil)) at 3 by (rewrite <- resize_succ; apply resize_length_eq; auto).
+        rewrite <- app_assoc. reflexivity.
+  Qed.
+
+  Definition project (np : nat * polyhedron) : imp polyhedron :=
+    let (n, p) := np in
+    let k := poly_nrl p in
+    do_project n (k - n)%nat p.
+
+  Lemma project_in_iff :
+    forall s n p pol, 0 < s -> WHEN proj <- project (n, pol) THEN
+                              in_poly p (expand_poly s proj) = true <->
+                         exists t m, 0 < t /\ in_poly (resize n (mult_vector t p) ++ m) (expand_poly (s * t) pol) = true.
+  Proof.
+    intros s n p pol Hs proj Hproj.
+    unfold project in Hproj.
+    remember (poly_nrl pol) as u.
+    rewrite (do_project_in_iff _ _ _ _ _ Hs _ Hproj).
+    split.
+    - intros [t [m [Hmlen [Ht Hin]]]]; exists t. exists m. split; [auto|].
+      rewrite <- in_poly_nrlength with (n := u) in Hin by (rewrite expand_poly_nrl; nia).
+      rewrite <- in_poly_nrlength with (n := u) by (rewrite expand_poly_nrl; nia).
+      rewrite app_assoc in Hin. rewrite resize_app_ge in Hin; [exact Hin|].
+      rewrite app_length, resize_length, Hmlen. lia.
+    - intros [t [m [Ht Hin]]]; exists t. exists (resize (u - n)%nat m).
+      split; [apply resize_length|]. split; [auto|].
+      rewrite <- in_poly_nrlength with (n := u) in Hin by (rewrite expand_poly_nrl; nia).
+      rewrite <- in_poly_nrlength with (n := u) by (rewrite expand_poly_nrl; nia).
+      rewrite app_assoc, resize_app_ge by (rewrite app_length, !resize_length; lia).
+      destruct (u <=? n)%nat eqn:Hun; reflect.
+      + rewrite resize_app_ge in * by (rewrite resize_length; lia). exact Hin.
+      + rewrite resize_app_le in * by (rewrite resize_length; lia). rewrite !resize_length in *.
+        rewrite resize_resize; [exact Hin|lia].
+  Qed.
+
+  Lemma project_in_iff1 :
+    forall n p pol, WHEN proj <- project (n, pol) THEN
+                    in_poly p proj = true <->
+               exists t m, 0 < t /\ in_poly (resize n (mult_vector t p) ++ m) (expand_poly t pol) = true.
+  Proof.
+    intros n p pol proj Hproj.
+    rewrite <- expand_poly_1 with (p := proj).
+    assert (H01 : 0 < 1) by lia.
+    rewrite (project_in_iff _ _ _ _ H01 _ Hproj). apply exists_ext. intros t.
+    destruct t; reflexivity.
+  Qed.
+
+  Theorem project_inclusion :
+    forall n p pol, in_poly p pol = true -> WHEN proj <- project (n, pol) THEN in_poly (resize n p) proj = true.
+  Proof.
+    intros n p pol Hp proj Hproj.
+    rewrite (project_in_iff1 _ _ _ _ Hproj). exists 1. exists (skipn n p).
+    split; [lia|].
+    rewrite mult_vector_1, resize_resize, resize_skipn_eq, expand_poly_1 by lia.
+    auto.
+  Qed.
+
+  Definition project_invariant n p v :=
+    exists t m, 0 < t /\ in_poly (resize n (mult_vector t v) ++ m) (expand_poly t p) = true.
+
+  Theorem project_invariant_inclusion :
+    forall n pol p, in_poly p pol = true -> project_invariant n pol (resize n p).
+  Proof.
+    intros n pol p H.
+    exists 1. exists (skipn n p).
+    split; [lia|].
+    rewrite mult_vector_1, resize_resize, resize_skipn_eq, expand_poly_1 by lia.
+    auto.
+  Qed.
+
+  Theorem project_id :
+    forall n pol p, (forall c, In c pol -> fst c =v= resize n (fst c)) -> project_invariant n pol p -> in_poly p pol = true.
+  Proof.
+    intros n pol p Hclen Hinv. rewrite poly_nrl_def in Hclen.
+    destruct Hinv as [t [m [Ht Hinv]]].
+    rewrite <- in_poly_nrlength with (n := n) in Hinv by (rewrite expand_poly_nrl; auto; lia).
+    rewrite resize_app in Hinv by (apply resize_length).
+    rewrite in_poly_nrlength in Hinv by (rewrite expand_poly_nrl; auto; lia).
+    rewrite expand_poly_eq in Hinv; auto.
+  Qed.
+
+  Theorem project_invariant_resize :
+    forall n pol p, project_invariant n pol p <-> project_invariant n pol (resize n p).
+  Proof.
+    intros n pol p. unfold project_invariant.
+    apply exists_ext. intros t.
+    rewrite <- mult_vector_resize. rewrite resize_resize by lia.
+    reflexivity.
+  Qed.
+
+  Lemma do_project_no_new_var :
+    forall k d pol n, (forall c, In c pol -> nth n (fst c) 0 = 0) -> WHEN proj <- do_project d k pol THEN (forall c, In c proj -> nth n (fst c) 0 = 0).
+  Proof.
+    induction k.
+    - intros; simpl in *. xasimplify eauto.
+    - intros; simpl in *. xasimplify eauto.
+      generalize (Proj.project_no_new_var _ _ _ H _ Hexta). intros H1.
+      generalize (Canon.canonize_no_new_var _ _ H1 _ Hexta0). intros H2.
+      apply (IHk _ _ _ H2 _ Hexta1).
+  Qed.
+
+  Lemma do_project_constraints :
+    forall k d pol n, (d <= n < d + k)%nat -> WHEN proj <- do_project d k pol THEN (forall c, In c proj -> nth n (fst c) 0 = 0).
+  Proof.
+    induction k.
+    - intros; lia.
+    - intros d pol n Hn proj Hproj.
+      simpl in Hproj.
+      bind_imp_destruct Hproj proja Hproja.
+      bind_imp_destruct Hproj canon Hcanon.
+      destruct (n =? d + k)%nat eqn:Heqn; reflect.
+      + rewrite Heqn. generalize (Proj.project_projected _ _ _ Hproja). intros H1.
+        generalize (Canon.canonize_no_new_var _ _ H1 _ Hcanon). intros H2.
+        apply (do_project_no_new_var _ _ _ _ H2 _ Hproj).
+      + assert (H : (d <= n < d + k)%nat) by lia.
+        apply (IHk _ _ _ H _ Hproj).
+  Qed.
+
+  Theorem project_constraint_size :
+    forall n pol c, WHEN proj <- project (n, pol) THEN In c proj -> fst c =v= resize n (fst c).
+  Proof.
+    intros n pol c proj Hproj Hin.
+    apply vector_nth_veq. intros k.
+    unfold project in Hproj.
+    rewrite nth_resize.
+    destruct (k <? n)%nat eqn:Hkn; reflect; [reflexivity|].
+    destruct (k <? n + (poly_nrl pol - n))%nat eqn:Hkrl; reflect.
+    - apply (do_project_constraints _ _ _ _ (conj Hkn Hkrl) _ Hproj); auto.
+    - assert (Hnrl : (poly_nrl pol <= k)%nat) by lia.
+      rewrite <- poly_nrl_def in Hnrl.
+      assert (H : forall c, In c pol -> nth k (fst c) 0 = 0).
+      + intros c1 Hin1; specialize (Hnrl c1 Hin1).
+        apply nth_eq with (n := k) in Hnrl. rewrite nth_resize in Hnrl. destruct (k <? k)%nat eqn:Hkk; reflect; lia.
+      + apply (do_project_no_new_var _ _ _ _  H _ Hproj _ Hin).
+  Qed.
+
+  Theorem project_next_r_inclusion :
+    forall n pol p, project_invariant n pol p ->
+               WHEN proj <- project (S n, pol) THEN
+               (forall c, In c proj -> nth n (fst c) 0 <> 0 -> satisfies_constraint p c = true) ->
+               project_invariant (S n) pol p.
+  Proof.
+    intros n pol p Hinv proj Hproj Hsat.
+    destruct Hinv as [t [m [Ht Hinv]]].
+    apply (project_in_iff1 _ _ _ _ Hproj).
+    unfold in_poly. rewrite forallb_forall. intros c Hinproj.
+    destruct (nth n (fst c) 0 =? 0) eqn:Hzero; reflect; [|apply Hsat; auto].
+    unfold project_invariant in Hinv.
+    rewrite <- resize_skipn_eq with (d := 1%nat) (l := m) in Hinv.
+    rewrite app_assoc in Hinv.
+    assert (H : in_poly (resize n (mult_vector t p) ++ resize 1 m) (expand_poly t proj) = true).
+    - rewrite (project_in_iff _ _ _ _ Ht _ Hproj). exists 1. exists (skipn 1%nat m).
+      split; [lia|]. rewrite mult_vector_1. rewrite resize_length_eq by (rewrite app_length, !resize_length; lia).
+      rewrite Z.mul_1_r; apply Hinv.
+    - unfold in_poly in H. rewrite forallb_forall in H.
+      rewrite <- mult_constraint_cst_eq with (k := t) by auto.
+      specialize (H (mult_constraint_cst t c)).
+      generalize (project_constraint_size _ _ _ _ Hproj Hinproj); intros Hsize.
+      rewrite resize_succ, Hzero in Hsize.
+      setoid_replace (0 :: nil) with (@nil Z) using relation veq in Hsize by (rewrite <- is_eq_veq; reflexivity).
+      rewrite app_nil_r in Hsize. symmetry in Hsize; rewrite nrlength_def in Hsize.
+      replace (fst c) with (fst (mult_constraint_cst t c)) in Hsize by reflexivity.
+      rewrite <- satisfies_constraint_nrlength with (n := n) in H by auto.
+      rewrite <- satisfies_constraint_nrlength with (n := n) by auto.
+      rewrite resize_app in H by (apply resize_length). apply H.
+      unfold expand_poly. apply in_map. auto.
+  Qed.
+
+  Definition project_invariant_export (np : nat * polyhedron) : imp polyhedron :=
+    project np.
+
+  Theorem project_invariant_export_correct :
+    forall n p pol, WHEN res <- project_invariant_export (n, pol) THEN in_poly p res = true <-> project_invariant n pol p.
+  Proof.
+    intros n p pol proj Hproj.
+    apply (project_in_iff1 _ _ _ _ Hproj).
+  Qed.
+
+End PolyProjectImpl.
+
+(*
 Module PolyProjectVPL (Dom : HasAssume QNum Cstr BasicD) <: PolyProject.
 
   Axiom extractImp : forall A, imp A -> A.
@@ -454,36 +1148,31 @@ Module PolyProjectVPL (Dom : HasAssume QNum Cstr BasicD) <: PolyProject.
   Theorem project_inclusion :
     forall n p pol proj, project n pol = Ok proj -> in_poly p pol = true -> in_poly (resize n p) proj = true.
   Proof.
-  Qed.
+  Admitted.
 
   Definition project_invariant n pol p :=
     forall c, In c pol -> fst c =v= resize n (fst c) -> satisfies_constraint p c = true.
 
-  Theorem project_reverse_inclusion :
-    forall n pol proj c, project n pol = Ok proj -> In c pol -> fst c =v= resize n (fst c) -> (exists c', c =c= c' /\ In c' proj).
-  Proof.
-  Qed.
-
   Theorem project_invariant_inclusion :
     forall n pol p, in_poly p pol = true -> project_invariant n pol (resize n p).
   Proof.
-  Qed.
+  Admitted.
 
   Theorem project_id :
     forall n pol p, (forall c, In c pol -> fst c =v= resize n (fst c)) -> project_invariant n pol p -> in_poly p pol = true.
   Proof.
-  Qed.
+  Admitted.
 
   Theorem project_next_r_inclusion :
     forall n pol proj p, project (S n) pol = Ok proj -> project_invariant n pol p ->
                     (forall c, In c proj -> nth n (fst c) 0 <> 0 -> satisfies_constraint p c = true) -> project_invariant (S n) pol p.
   Proof.
-  Qed.
+  Admitted.
 
   Theorem project_invariant_resize :
     forall n pol p, project_invariant n pol p <-> project_invariant n pol (resize n p).
   Proof.
-  Qed.
+  Admitted.
 
   Definition project_invariant_export n (pol : polyhedron) :=
     Ok (filter (fun c => is_eq (fst c) (resize n (fst c))) pol).
@@ -491,16 +1180,22 @@ Module PolyProjectVPL (Dom : HasAssume QNum Cstr BasicD) <: PolyProject.
   Theorem project_invariant_export_correct :
     forall n p pol res, project_invariant_export n pol = Ok res -> in_poly p res = true <-> project_invariant n pol p.
   Proof.
-  Qed.
+  Admitted.
 
   Theorem project_constraint_size :
     forall n pol proj c, project n pol = Ok proj -> In c proj -> fst c =v= resize n (fst c).
   Proof.
-  Qed.
+  Admitted.
 
 End PolyProjectVPL.
+ *)
 
-Import PolyProjectSimple.
+Import CoreAlarmed.
+Module PPS := PolyProjectSimple CoreAlarmed.
+Import PPS.
+Global Opaque project.
+Ltac bind_imp_destruct H id1 id2 :=
+  apply mayReturn_bind in H; destruct H as [id1 [id2 H]].
 
 (*
 Theorem project_id :
@@ -532,15 +1227,30 @@ Admitted.
 
 (** * Generating the code *)
 
-Fixpoint generate_loop (d : nat) (n : nat) (pi : Polyhedral_Instruction) : result stmt :=
+Definition res_to_alarm {A : Type} (d : A) (x : result A) : imp A :=
+  match x with
+  | Ok a => pure a
+  | Err s => alarm s d
+  end.
+
+Lemma res_to_alarm_correct :
+  forall (A : Type) (d : A) (x : result A) (y : A),
+    mayReturn (res_to_alarm d x) y -> x = Ok y.
+Proof.
+  intros A d x y. destruct x; simpl.
+  - intros H. f_equal. apply mayReturn_pure. auto.
+  - intros H. apply mayReturn_alarm in H. tauto.
+Qed.
+
+Fixpoint generate_loop (d : nat) (n : nat) (pi : Polyhedral_Instruction) : imp stmt :=
   match d with
-  | O => Ok (Instr pi.(pi_instr) (map (make_affine_expr n) pi.(pi_transformation)))
+  | O => pure (Instr pi.(pi_instr) (map (make_affine_expr n) pi.(pi_transformation)))
   | S d1 =>
-    do proj <- project (n - d1)%nat pi.(pi_poly) ;
-    do lb <- find_lower_bound (n - d)%nat proj ;
-    do ub <- find_upper_bound (n - d)%nat proj ;
-    do inner <- generate_loop d1 n pi ;
-    Ok (Loop lb ub inner)
+    BIND proj <- project ((n - d1)%nat, pi.(pi_poly)) -;
+    BIND lb <- res_to_alarm (Constant 0) (find_lower_bound (n - d)%nat proj) -;
+    BIND ub <- res_to_alarm (Constant 0) (find_upper_bound (n - d)%nat proj) -;
+    BIND inner <- generate_loop d1 n pi -;
+    pure (Loop lb ub inner)
   end.
 
 Lemma env_scan_begin :
@@ -588,15 +1298,15 @@ Proof.
 Qed.
 
 Lemma generate_loop_single_point :
-  forall n pi st env mem1 mem2,
-    generate_loop 0%nat n pi = Ok st ->
+  forall n pi env mem1 mem2,
+    WHEN st <- generate_loop 0%nat n pi THEN
     loop_semantics st env mem1 mem2 ->
     length env = n ->
     in_poly (rev env) pi.(pi_poly) = true ->
     env_poly_lex_semantics (rev env) n (pi :: nil) mem1 mem2.
 Proof.
-  intros n pi st env mem1 mem2 Hgen Hsem Hlen Henvsat. simpl in *.
-  injection Hgen as Hgen.
+  intros n pi env mem1 mem2 st Hgen Hsem Hlen Henvsat. simpl in *.
+  apply mayReturn_pure in Hgen.
   unfold env_poly_lex_semantics.
   eapply PolyLexProgress with (n := 0%nat) (p := rev env); [ |reflexivity| | | apply PolyLexDone].
   - unfold env_scan. simpl. reflect. split; [split|].
@@ -618,44 +1328,17 @@ Proof.
     destruct H2; congruence.
 Qed.
 
-(*
-Lemma satisfies_extend :
-  forall n pol proj lb ub env x,
-    length env = n ->
-    (forall c, In c pol -> fst c =v= resize n (fst c) -> satisfies_constraint (rev env) c = true) ->
-    project (S n) pol = Ok proj ->
-    find_lower_bound n proj = Ok lb ->
-    find_upper_bound n proj = Ok ub ->
-    eval_expr env lb <= x < eval_expr env ub ->
-    (forall c, In c pol -> fst c =v= resize (S n) (fst c) -> satisfies_constraint (rev env ++ x :: nil) c = true).
-Proof.
-  intros n pol proj lb ub env x Hlen Hsat Hproj Hlb Hub Hx c Hin Hsize.
-  destruct (project_reverse_inclusion (S n) pol proj c Hproj Hin Hsize) as [c' [Heqc' Hinc']].
-  rewrite resize_succ in Hsize.
-  destruct (nth n (fst c) 0 =? 0) eqn:Hzero; reflect.
-  - rewrite Hzero in Hsize.
-    setoid_replace (0 :: nil) with (@nil Z) in Hsize by (rewrite <- is_eq_veq; auto).
-    unfold satisfies_constraint. rewrite Hsize.
-    rewrite dot_product_app by (rewrite rev_length, resize_length; auto). simpl.
-    rewrite Z.add_0_r. rewrite app_nil_r in Hsize.
-    rewrite <- Hsize. apply Hsat; auto.
-  - rewrite Heqc'. rewrite find_bounds_correct in Hx by eauto.
-    apply Hx; auto. erewrite nth_eq in Hzero; [exact Hzero|].
-    rewrite Heqc'; reflexivity.
-Qed.
- *)
-
 Lemma env_scan_extend :
-  forall d n pi proj lb ub env m p,
+  forall d n pi lb ub env m p,
     length env = n ->
     (n < d)%nat ->
-    project (S n) pi.(pi_poly) = Ok proj ->
+    WHEN proj <- project (S n, pi.(pi_poly)) THEN
     find_lower_bound n proj = Ok lb ->
     find_upper_bound n proj = Ok ub ->
     env_scan (pi :: nil) (rev env) d m p =
       existsb (fun x : Z => env_scan (pi :: nil) (rev env ++ x :: nil) d m p) (Zrange (eval_expr env lb) (eval_expr env ub)).
 Proof.
-  intros d n pi proj lb ub env m p Hlen Hnd Hproj Hlb Hub.
+  intros d n pi lb ub env m p Hlen Hnd proj Hproj Hlb Hub.
   rewrite eq_iff_eq_true. rewrite existsb_exists.
   rewrite env_scan_split by (rewrite rev_length; lia).
   split.
@@ -665,9 +1348,9 @@ Proof.
     destruct Hscan as [[Hscan1 Hscan2] Hscan3].
     assert (Hinproj : in_poly (rev env ++ x :: nil) proj = true).
     {
-      rewrite Hscan1. eapply project_inclusion; [|apply Hscan3].
-      rewrite app_length; rewrite rev_length; rewrite Hlen; simpl.
-      rewrite <- Hproj. f_equal. lia.
+      rewrite Hscan1. eapply project_inclusion; [apply Hscan3|].
+      rewrite app_length; rewrite rev_length; rewrite Hlen; unfold length.
+      replace (n + 1)%nat with (S n) by lia. apply Hproj.
     }
     rewrite find_bounds_correct by eauto.
     unfold in_poly in Hinproj. rewrite forallb_forall in Hinproj.
@@ -676,9 +1359,9 @@ Proof.
 Qed.
 
 Theorem generate_loop_preserves_sem :
-  forall d n pi st env mem1 mem2,
+  forall d n pi env mem1 mem2,
     (d <= n)%nat ->
-    generate_loop d n pi = Ok st ->
+    WHEN st <- generate_loop d n pi THEN
     loop_semantics st env mem1 mem2 ->
     length env = (n - d)%nat ->
     (forall c, In c pi.(pi_poly) -> fst c =v= resize n (fst c)) ->
@@ -686,13 +1369,16 @@ Theorem generate_loop_preserves_sem :
     env_poly_lex_semantics (rev env) n (pi :: nil) mem1 mem2.
 Proof.
   induction d.
-  - intros n pi st env mem1 mem2 Hnd Hgen Hsem Hlen Hpilen Hinv.
+  - intros n pi env mem1 mem2 Hnd st Hgen Hsem Hlen Hpilen Hinv.
     eapply generate_loop_single_point; eauto; try lia.
     eapply project_id; eauto.
     rewrite Nat.sub_0_r in Hinv. auto.
-  - intros n pi st env mem1 mem2 Hnd Hgen Hsem Hlen Hpilen Hinv. simpl in *.
-    bind_ok_destruct Hgen proj Hproj. bind_ok_destruct Hgen lb Hlb. bind_ok_destruct Hgen ub Hub. bind_ok_destruct Hgen inner Hinner.
-    injection Hgen as Hgen. rewrite <- Hgen in Hsem.
+  - intros n pi env mem1 mem2 Hnd st Hgen Hsem Hlen Hpilen Hinv. simpl in *.
+    bind_imp_destruct Hgen proj Hproj.
+    bind_imp_destruct Hgen lb Hlb. apply res_to_alarm_correct in Hlb.
+    bind_imp_destruct Hgen ub Hub. apply res_to_alarm_correct in Hub.
+    bind_imp_destruct Hgen inner Hinner.
+    apply mayReturn_pure in Hgen. rewrite <- Hgen in Hsem.
     inversion_clear Hsem.
     unfold env_poly_lex_semantics in *.
     eapply poly_lex_semantics_extensionality.
@@ -700,7 +1386,7 @@ Proof.
       * eapply iter_semantics_map; [|apply H]. simpl.
         intros x mem3 mem4 Hbounds Hloop. eapply IHd with (env := x :: env); simpl; eauto; try lia.
         replace (n - d)%nat with (S (n - S d))%nat in * by lia.
-        eapply project_next_r_inclusion; [exact Hproj| |].
+        eapply project_next_r_inclusion; [|exact Hproj|].
         -- rewrite project_invariant_resize. rewrite resize_app by (rewrite rev_length; auto).
            apply Hinv.
         -- rewrite <- find_bounds_correct; eauto.
@@ -720,23 +1406,7 @@ Proof.
         rewrite lex_compare_reflexive in Hcmp. simpl in Hcmp.
         destruct (x2 ?= x1) eqn:Hcmpx; reflect; [lia | lia | congruence].
     + simpl. intros m p. erewrite env_scan_extend; eauto; try lia.
-      rewrite <- Hproj; f_equal; lia.
-Qed.
-
-Fixpoint list_max l :=
-  match l with
-  | nil => 0%nat
-  | x :: l => Nat.max x (list_max l)
-  end.
-
-Theorem list_max_le :
-  forall l n, (list_max l <= n -> (forall x, In x l -> x <= n))%nat.
-Proof.
-  induction l; simpl in *.
-  - intros; exfalso; auto.
-  - intros n H x [Ha | Hl].
-    + lia.
-    + apply IHl; auto; lia.
+      replace (S (n - S d)) with (n - d)%nat by lia. apply Hproj.
 Qed.
 
 Fixpoint and_all l :=
@@ -748,8 +1418,8 @@ Fixpoint and_all l :=
 Theorem and_all_correct :
   forall l env, eval_test env (and_all l) = forallb (eval_test env) l.
 Proof.
-  induction l; simpl in *; auto.
-(*  intros; rewrite IHl; auto. *)
+  induction l; simpl in *; [auto|].
+  intros; rewrite IHl; auto.
 Qed.
 
 Definition make_affine_test n c := LE (make_linear_expr n (fst c)) (Constant (snd c)).
@@ -773,41 +1443,26 @@ Proof.
   rewrite forallb_map. apply forallb_ext. intros c. apply make_affine_test_correct. auto.
 Qed.
 
-(*
-Definition make_smalldims_test d n poly :=
-  and_all (map (make_affine_test n) (filter (fun c => is_eq (fst c) (resize d (fst c))) poly)).
-
-Lemma make_smalldims_test_correct :
-  forall d n poly env, length env = n ->
-                  eval_test env (make_smalldims_test d n poly) = true <->
-                  (forall c, In c poly -> fst c =v= resize d (fst c) -> satisfies_constraint (rev env) c = true).
-Proof.
-  intros d n poly env Hlen.
-  unfold make_smalldims_test. rewrite and_all_correct. rewrite forallb_map. rewrite forallb_forall.
-  apply forall_ext. intros c. rewrite make_affine_test_correct by auto.
-  rewrite filter_In. tauto.
-Qed.
- *)
-
 Definition generate d n pi :=
-  do st <- generate_loop d n pi ;
-  do ctx <- project_invariant_export (n - d)%nat pi.(pi_poly) ;
-  Ok (Guard (make_poly_test (n - d)%nat ctx) st).
+  BIND st <- generate_loop d n pi -;
+  BIND ctx <- project_invariant_export ((n - d)%nat, pi.(pi_poly)) -;
+  pure (Guard (make_poly_test (n - d)%nat ctx) st).
 
 Theorem generate_preserves_sem :
-  forall d n pi st env mem1 mem2,
+  forall d n pi env mem1 mem2,
     (d <= n)%nat ->
-    generate d n pi = Ok st ->
+    WHEN st <- generate d n pi THEN
     loop_semantics st env mem1 mem2 ->
     length env = (n - d)%nat ->
     (forall c, In c pi.(pi_poly) -> fst c =v= resize n (fst c)) ->
     env_poly_lex_semantics (rev env) n (pi :: nil) mem1 mem2.
 Proof.
-  intros d n pi st env mem1 mem2 Hd Hgen Hloop Henv Hsize.
-  bind_ok_destruct Hgen st1 H. bind_ok_destruct Hgen ctx Hctx. injection Hgen as Hgen.
+  intros d n pi env mem1 mem2 Hd st Hgen Hloop Henv Hsize.
+  bind_imp_destruct Hgen st1 H. bind_imp_destruct Hgen ctx Hctx.
+  apply mayReturn_pure in Hgen.
   rewrite <- Hgen in *. inversion_clear Hloop.
   - eapply generate_loop_preserves_sem; eauto.
-    rewrite <- project_invariant_export_correct by eauto.
+    rewrite <- (project_invariant_export_correct _ _ _ _ Hctx) by eauto.
     erewrite <- make_poly_test_correct; [|apply Henv]. auto.
   - apply PolyLexDone. intros n0 p. unfold env_scan.
     destruct n0; simpl in *; [|destruct n0]; auto. reflect.
@@ -816,9 +1471,21 @@ Proof.
     destruct (is_eq (rev env) (resize (n - d)%nat p)) eqn:Hpenv; auto.
     destruct (in_poly p pi.(pi_poly)) eqn:Hpin; auto. exfalso.
     eapply project_invariant_inclusion in Hpin.
-    rewrite <- project_invariant_export_correct in Hpin; [|exact Hctx].
+    rewrite <- (project_invariant_export_correct _ _ _ _ Hctx) in Hpin.
     reflect. rewrite <- Hpenv in Hpin. congruence.
 Qed.
+
+
+
+
+
+
+
+
+
+
+
+
 
 (*
 Definition generate es pi :=
